@@ -20,48 +20,51 @@ public inductive SplitNode
   | Split (varIndex: USize) (bitIndex: Nat) (left: SplitNode) (right: SplitNode)
 deriving Repr
 
-def Assignment2 := Array (EvalValue Bitvector)
-def Assignment3 := Array (EvalValue Bitvector3)
+def Assignment2 := Assignment Bitvector
+def Assignment3 := Assignment Bitvector3
 
-def checkNode (formula: Formula) (assignment: Assignment3) (node: SplitNode) : Except EChecker (Option Bool) :=
+def checkNode (formula: Formula 1) (assignment: Assignment3) (node: SplitNode) : Except EChecker (Option Bool) :=
   match node with
     | SplitNode.Leaf =>
       (eval3 formula assignment).mapError EChecker.Evaluator
     | SplitNode.Split varIndex bitIndex left right =>
-      if hx: varIndex.toNat < assignment.size then
-        let varAssignment := assignment.uget varIndex hx
+      if hx: varIndex.toNat < assignment.inner.size then
+
+        let varAssignment := assignment.inner.uget varIndex hx
         let (leftSplit, rightSplit) := varAssignment.value.split bitIndex
+
 
         let leftSplit: EvalValue Bitvector3 := { width := varAssignment.width, value := leftSplit }
 
         if let some rightSplit := rightSplit then
           let rightSplit: EvalValue Bitvector3 := { width := varAssignment.width, value := rightSplit }
 
-          let leftAssignment := assignment.uset varIndex leftSplit hx
-          let rightAssignment := assignment.uset varIndex rightSplit hx
+          let leftAssignment := { inner := assignment.inner.uset varIndex leftSplit hx }
+          let rightAssignment := { inner := assignment.inner.uset varIndex rightSplit hx }
           match checkNode formula leftAssignment left, checkNode formula rightAssignment right with
             | Except.ok (some left), Except.ok (some right) => Except.ok (some (left || right))
             | Except.ok _, Except.ok _ => Except.ok none
             | Except.error err, _ | _, Except.error err => Except.error err
         else
-          let leftAssignment := assignment.uset varIndex leftSplit hx
+          let leftAssignment := { inner := assignment.inner.uset varIndex leftSplit hx }
           checkNode formula leftAssignment left
+
       else
         Except.error (EChecker.BadSplitVariable varIndex)
 
 def Assignment3.containsConcrete (abstract: Assignment3) (concrete: Assignment2) : Bool :=
+  let abstract := abstract.inner
+  let concrete := concrete.inner
   if abstract.size == concrete.size then
     (abstract.zip concrete).all (λ (abstract, concrete) =>
-      if concrete.width = abstract.width then
-        let v: Bitvector abstract.width :=
+        let concreteValue: Bitvector abstract.width :=
           { value := BitVec.ofNat abstract.width (BitVec.toNat concrete.value.value)}
-        AbstractDomain.containsConcrete abstract.value v
-      else
-        false
+        AbstractDomain.containsConcrete abstract.value concreteValue
     )
   else
     false
 
+/-
 theorem domain_sound
   (formula: Formula) (abstract: Assignment3) (concrete: Assignment2) (result: Bool)
   : eval3 formula abstract = Except.ok (some result) →
@@ -123,21 +126,24 @@ theorem checkNode_sound (formula: Formula) (node: SplitNode)
 
     contradiction -- bad split variable
   }
+-/
+
+public def check (variables: Array BitvectorType) (formula: Formula 1) (splitTree: SplitNode) : Except EChecker (Option Bool) := do
+  let foldFn := fun array e => array.push { width := e.width, value := Bitvector3.allUnknown e.width }
+
+  let array := variables.foldl foldFn #[]
+
+  let assignment: Assignment3 := { inner := array }
+
+  checkNode formula assignment splitTree
 
 
-public def check (problem: Problem) (splitTree: SplitNode) : Except EChecker (Option Bool) := do
-  let mut assignment := problem.variables.foldl
-    (λ array e => array.push ({ width := e.width, value := Bitvector3.allUnknown e.width })) #[]
-
-  checkNode problem.formula assignment splitTree
-
-
-public def solve (problem: Problem) : Except EChecker (Option Bool) := do
+public def solve (variables: Array BitvectorType) (formula: Formula 1) : Except EChecker (Option Bool) := do
   let mut splitTree := SplitNode.Leaf
   let mut varIndex := 0
-  for var in problem.variables do
+  for var in variables do
     for bitIndex in 0...var.width do
       splitTree := SplitNode.Split varIndex bitIndex splitTree splitTree
     varIndex := varIndex + 1
 
-  check problem splitTree
+  check variables formula splitTree
